

Maclaurin & Taylor Series formula

$$\sum_{n=0}^{\infty} \frac{f^{(n)}(a)}{n!} \cdot (x-a)^n$$

a = real or complex number

$f^{(n)}(a)$ = n^{th} derivative of f evaluated at the Point a .

By using the above expansion formula

$$\sin x = x - \frac{x^3}{3!} + \frac{x^5}{5!} - \frac{x^7}{7!} + \dots$$

$$\frac{\sin x}{x} = 1 - \frac{x^2}{3!} + \frac{x^4}{5!} - \frac{x^6}{7!} + \dots$$

Let,

$$f(x) = \frac{\sin x}{x} = 1 - \frac{x^2}{3!} + \frac{x^4}{5!} - \frac{x^6}{7!} + \dots$$

WKT,

Every polynomial can be represented as

$$f(x) = (a + x_1)(b + x_2) \dots \text{degree of the Polynomial times.}$$

as per roots of $\sin x/x$. (general)

$$f(x) = (\lambda)(x-\pi)(x+\pi)(x-2\pi)(x+2\pi)\dots \quad \text{--- (1)}$$

$$\frac{\sin x}{x} = 1 - \frac{x^2}{3!} + \frac{x^4}{5!} - \frac{x^6}{7!} \dots \quad \text{--- (2)}$$

The constant term from Expansion of (1)

is $\lambda(-\pi)(\pi)(2\pi)(-2\pi)\dots$

& from (2) is '1'

$$\Rightarrow \lambda(-\pi)(\pi)(2\pi)(-2\pi)\dots = 1$$

$$\lambda = \frac{1}{(-\pi)(\pi)(2\pi)(-2\pi)\dots}$$

$$f(x) = \lambda \cdot \pi \left(1 - \frac{x}{\pi}\right) \left(1 + \frac{x}{\pi}\right) (-\pi) (-2\pi) \left(1 - \frac{x}{2\pi}\right) \dots$$

$$f(x) = \lambda ((\pi)(-\pi)(2\pi)(-2\pi)\dots) \left(1 - \frac{x}{\pi}\right) \left(1 + \frac{x}{\pi}\right) \dots$$

$$f(x) = \lambda \cdot \frac{1}{\lambda} \cdot \left(1 - \frac{x}{\pi}\right) \left(1 + \frac{x}{\pi}\right) \left(1 - \frac{x}{2\pi}\right) \dots$$

$$f(x) = \left(1 - \frac{x^2}{\pi^2}\right) \left(1 - \frac{x^2}{4\pi^2}\right) \left(1 - \frac{x^2}{9\pi^2}\right) \dots$$

$$f(x) = \text{co-eff}(x^2) + \text{remaining terms.}$$

$$g(x) = -\frac{1}{\pi^2} - \frac{1}{4\pi^2} - \frac{1}{9\pi^2} - \dots = \text{co-eff}(x^2)$$

$$g'(x) = \left(\sum_{n=1}^{\infty} \frac{1}{n^2} \right) \left(-\frac{1}{\pi^2} \right) = -\frac{1}{3!} \quad \left[\text{from eq (2)} \right]$$

$$\sum_{n=1}^{\infty} \frac{1}{n^2} = \left(-\frac{1}{6}\right)(-\pi^2) = \frac{\pi^2}{6}$$

$$g(2) = \sum_{n=1}^{\infty} \frac{1}{n^2} = \frac{22 \times 22}{49 \times 6} = \frac{484}{49 \times 6} = 1.646$$

$$\frac{29}{18} < 1.646 < \frac{31}{18}$$

$$1.6\overline{11} < 1.646 < 1.7\overline{22}$$

which is equals to $\frac{1}{2} - \lim_{n \rightarrow \infty} \frac{1}{n^2 + n + 1}$

$$y = \frac{1}{2} - \lim_{n \rightarrow \infty} \left(\frac{1}{n^2} \left(1 + \frac{1}{n} + \frac{1}{n^2} \right) \right)$$

$\frac{1}{n} \rightarrow 0$ $\frac{1}{n^2} \rightarrow 0$ $\underbrace{\quad}_{l_1}$ $\underbrace{\quad}_{l_2}$

$$\frac{1}{2} - \lim_{n \rightarrow \infty} (0) \left(\frac{1}{1+0+0} \right)$$

Let,

$$\lim_{n \rightarrow \infty} l_1 = \lim_{n \rightarrow \infty} \frac{1}{n^2} = 0$$

$$\lim_{n \rightarrow \infty} l_2 = \lim_{n \rightarrow \infty} \frac{1}{1 + \frac{1}{n} + \frac{1}{n^2}}$$

$\underbrace{\quad}_{l_3}$ $\underbrace{\quad}_{l_4}$ $\underbrace{\quad}_{l_5}$

$$\lim_{n \rightarrow \infty} l_3 = \lim_{n \rightarrow \infty} 1 = 1$$

$$\lim_{n \rightarrow \infty} l_4 = \lim_{n \rightarrow \infty} \frac{1}{n} = 0$$

$$\lim_{n \rightarrow \infty} l_5 = \lim_{n \rightarrow \infty} \frac{1}{n^2} = 0$$

By the properties of limits, wkt,

$$\lim_{n \rightarrow c} (l_1 + l_2) = \lim_{n \rightarrow c} l_1 + \lim_{n \rightarrow c} l_2$$

$$\lim_{n \rightarrow c} l_1 \cdot l_2 = \lim_{n \rightarrow c} l_1 \cdot \lim_{n \rightarrow c} l_2$$

$$y = \frac{1}{2} - (0) \left(\frac{1}{1+0+0} \right)$$

$$y = \frac{1}{2}$$

1. Sequence $\{a_n\}$

$$a_n - a_{n-2} \rightarrow 0 \text{ when,}$$

$$n \rightarrow \infty$$

$$b_n = \frac{a_n - a_{n-1}}{n} \quad \text{--- (1)}$$

$$\text{now, } b_{n-1} = \frac{a_{n-1} - a_{n-2}}{n-1}$$

$$b_{n+1} = \frac{a_{n+1} - a_n}{n+1}$$

$$b_{n-1} > \frac{a_{n-1} - a_{n-2}}{n} \quad \text{--- (2)}$$

$$b_{n+1} < \frac{a_{n+1} - a_n}{n} \quad \text{--- (3)}$$

(1) + (2)

$$b_n + b_{n-1} > \frac{a_n - a_{n-2}}{n}$$

$$b_n + b_{n+1} < \frac{a_{n+1} - a_{n-1}}{n} \quad \text{--- (4)}$$

$$\text{if } b_{n+1} + b_n < \frac{a_{n+1} - a_{n-1}}{n}$$

then,

$$b_n + b_{n-1} < \frac{a_n - a_{n-2}}{n-1}$$

then,

$$\frac{a_n - a_{n-2}}{n} < b_n + b_{n-1} < \frac{a_n - a_{n-2}}{n-1}$$

As $n \rightarrow \infty$, both

$$\frac{a_n - a_{n-2}}{n}, \frac{a_n - a_{n-2}}{n-1}$$

converges to 0 as $a_n - a_{n-2} \rightarrow 0$
when $n \rightarrow \infty$ and $\frac{1}{n}, \frac{1}{n-1} \rightarrow 0$

WKT, By properties of limits

$$\lim_{x \rightarrow c} l_1 \cdot l_2 = \lim_{x \rightarrow c} l_1 \cdot \lim_{x \rightarrow c} l_2$$

Hence, $b_n + b_{n-1} \rightarrow 0$ when $n \rightarrow \infty$

Let $c_{n-1} = b_n + b_{n-1}$

c_{n-1} converges to some x

$\forall \epsilon > 0 \exists N_0 \in \mathbb{N}$ s.t. $\forall (n-1) \geq N_0$

$$|b_n + b_{n-1} - x| < \epsilon \quad \text{--- (8)}$$

By Law of Trichotomy

1) $b_n > b_{n-1}$ 2) $b_n < b_{n-1}$

3) $b_n = b_{n-1}$

① & ③ $b_n \geq b_{n-1}$

$$|b_n + b_{n-1} - x| < \frac{\epsilon}{2}$$

$$|2b_{n-1} - x| \leq |b_n + b_{n-1} - x| < \frac{\epsilon}{2}$$

$$|b_n - b_{n-1}| = |b_n + b_{n-1} - x + x - 2b_{n-1}|$$

$$\leq |b_n + b_{n-1} - x| + |x - 2b_{n-1}|$$

$$< \frac{\epsilon}{2} + \frac{\epsilon}{2}$$

$$|b_n - b_{n-1}| < \epsilon$$

② $b_n < b_{n-1}$

$$b_n < b_{n-1}$$

$$|b_n + b_{n-1} - x| < \frac{\epsilon}{2}$$

$$|2b_n - x| < |b_n + b_{n-1} - x| < \frac{\epsilon}{2}$$

$$|b_{n-1} - b_n| = |b_{n-1} + b_n - x + x - 2b_n|$$

$$\leq |b_{n-1} + b_n - x| + |x - 2b_n|$$

$$< \frac{\epsilon}{2} + \frac{\epsilon}{2}$$

$$|b_n - b_{n-1}| < \epsilon$$

Hence $\forall \epsilon > 0 \exists N_0 \in \mathbb{N}$ s.t. $(n-1) \geq N_0$
 $|b_n - b_{n-1}| < \epsilon$

taking $m, n \in \mathbb{N}$

$$|b_m - b_n| \leq |b_m - b_{m-1}| + |b_{m-1} - b_{m-2}| + \dots + |b_n - b_{n+1}|$$

$$|b_n - b_{n-1}| < \frac{\epsilon}{m+n-1} \quad \forall (n-1) \geq N_0$$

$$|b_m - b_n| \leq \frac{\epsilon}{m+n-1} + \frac{\epsilon}{m+n-1} + \dots + \frac{\epsilon}{m+n-1}$$

$$|b_m - b_n| \leq \left(\frac{\epsilon}{m+n-1} \right) m+n-1$$

let $m = n+p$

then, $\forall \epsilon > 0 \exists N_0 \in \mathbb{N}$ s.t. $n \geq N_0$,
p starts with 1

$$|b_{n+p} - b_n| < \epsilon$$

hence b_n is a Cauchy sequence

then a Cauchy can be convergent

let b_n converge to M

(then) $\forall \epsilon > 0 \exists N_0 \in \mathbb{N}$ s.t. $\forall n \geq N_0$

$$|b_n - y| < \epsilon/2 \quad \text{--- (4)}$$

then

$$|b_{n+1} - y| < \epsilon/2 \quad \text{--- (5)}$$

from (4) & (5)

$$|b_n + b_{n+1} - y - y| < |b_n - y| + |b_{n+1} - y|$$

$$|b_n + b_{n+1} - 2y| < \epsilon \quad \text{by Triangle inequality}$$

$$\text{wkt, } |b_n + b_{n+1} - x| < \epsilon \quad [\text{from (8)}]$$

$$x = 2y$$

$$y = \frac{x}{2}$$

we know that $x = 0$

hence $y = 0$

$\therefore b_n$ is a convergent sequence which converges to 0.

4. fact $(1 + \frac{1}{n})^n \rightarrow e$ as $n \rightarrow \infty$

Since $x \rightarrow \infty$, we assume, $x > 1$

let $[x] = p$. Then $p \leq x < p+1$

$$\text{and } 1 + \frac{1}{p+1} < 1 + \frac{1}{x} \leq 1 + \frac{1}{p}$$

It follows that

$$\left(1 + \frac{1}{p+1}\right)^{p+1} < \left(1 + \frac{1}{x}\right)^x < \left(1 + \frac{1}{p}\right)^{p+1}$$

Taking limit as $x \rightarrow \infty$ and noting that as

$$x \rightarrow \infty, p \rightarrow \infty$$

$$\text{We have } \lim_{x \rightarrow \infty} \left(1 + \frac{1}{x}\right)^x \geq \lim_{p \rightarrow \infty} \left(1 + \frac{1}{p+1}\right)^{p+1}$$

$$= \lim_{p \rightarrow \infty} \frac{1}{\left(1 + \frac{1}{p+1}\right)^{p+1}} \left(1 + \frac{1}{p+1}\right)^{p+1} = e$$

$$\text{Also } \lim_{x \rightarrow \infty} \left(1 + \frac{1}{x}\right)^x \leq \lim_{p \rightarrow \infty} \left(1 + \frac{1}{p}\right)^{p+1}$$

$$= \lim_{p \rightarrow \infty} \left(1 + \frac{1}{p}\right)^p \cdot \left(1 + \frac{1}{p}\right) = e$$

It follows that $\lim_{x \rightarrow \infty} \left(1 + \frac{1}{x}\right)^x = e$.

2. $\lim_{n \rightarrow \infty} \sum_{k=1}^n \left(\sqrt{1 + \frac{k}{n^2}} - 1 \right)$

multiply and divide conjugate

$$\lim_{n \rightarrow \infty} \sum_{k=1}^n \frac{\left(\sqrt{1 + \frac{k}{n^2}} - 1 \right) \left(\sqrt{1 + \frac{k}{n^2}} + 1 \right)}{\left(\sqrt{1 + \frac{k}{n^2}} + 1 \right)}$$

$$\lim_{n \rightarrow \infty} \sum_{k=1}^n \left(\sqrt{1 + \frac{k}{n^2}} - 1 \right) \left(\frac{1}{\sqrt{1 + \frac{k}{n^2}} + 1} \right)$$

$$\lim_{n \rightarrow \infty} \sum_{k=1}^n \frac{k}{n^2} \left(\frac{1}{\sqrt{1 + \frac{k}{n^2}} + 1} \right)$$

Expanding

$$= \lim_{n \rightarrow \infty} \left(\frac{1}{n^2} \left(\frac{1}{\sqrt{1 + \frac{1}{n^2}} + 1} \right) + \frac{2}{n^2} \left(\frac{1}{\sqrt{1 + \frac{2}{n^2}} + 1} \right) \right. \\ \left. \dots + \frac{n}{n^2} \left(\frac{1}{\sqrt{1 + \frac{n}{n^2}} + 1} \right) \right)$$

when $n \rightarrow \infty$, $\frac{1}{n} \rightarrow 0$ and by limit

properties $\lim_{x \rightarrow c} f(x) \cdot g(x) = \lim_{x \rightarrow c} f(x) \cdot \lim_{x \rightarrow c} g(x)$

and $\lim_{x \rightarrow c} \frac{f(x)}{g(x)} = \frac{\lim_{x \rightarrow c} f(x)}{\lim_{x \rightarrow c} g(x)}$

$$= \lim_{n \rightarrow \infty} \left(\frac{1}{n^2} \left(\frac{1}{\sqrt{1+0} + 1} \right) + \frac{2}{n^2} \left(\frac{1}{\sqrt{1+0} + 1} \right) \right. \\ \left. \dots + \frac{n}{n^2} \left(\frac{1}{\sqrt{1+0} + 1} \right) \right)$$

$$\begin{aligned}
 & \left[\text{When } n \rightarrow \infty \quad \frac{1}{n^2}, \frac{2}{n^2}, \frac{3}{n^2}, \dots, \frac{n}{n^2} \rightarrow 0 \right] \\
 &= \lim_{n \rightarrow \infty} \left(\frac{1}{n^2} \left(\frac{1}{2} \right) + \frac{2}{n^2} \left(\frac{1}{2} \right) + \dots + \frac{n}{n^2} \left(\frac{1}{2} \right) \right) \\
 &= \frac{1}{2} \lim_{n \rightarrow \infty} \left(\frac{1}{n^2} + \frac{2}{n^2} + \dots + \frac{n}{n^2} \right) \\
 &= \frac{1}{2} \lim_{n \rightarrow \infty} \sum_{k=1}^n \left(\frac{k}{n^2} \right) \quad \left[\because \lim_{n \rightarrow c} f \cdot g = \left(\lim_{n \rightarrow c} f \right) \left(\lim_{n \rightarrow c} g \right) \right] \\
 &= \frac{1}{2} \lim_{n \rightarrow \infty} \left(\frac{1}{n^2} \left[\sum_{k=1}^n k \right] \right) \quad \left[\because \sum_{i=1}^n i = \frac{n(n+1)}{2} \right] \\
 &= \frac{1}{2} \lim_{n \rightarrow \infty} \left(\frac{1}{n^2} \left(\frac{n(n+1)}{2} \right) \right) \\
 &= \frac{1}{2 \cdot 2} \lim_{n \rightarrow \infty} \left[\frac{n^2 + n}{n^2} \right] \\
 &= \frac{1}{4} \cdot \lim_{n \rightarrow \infty} \left[1 + \frac{1}{n} \right] \quad \lim_{n \rightarrow c} (f+g) = \lim_{n \rightarrow c} f + \lim_{n \rightarrow c} g \\
 &= \frac{1}{4} \left[\lim_{n \rightarrow \infty} 1 + \lim_{n \rightarrow \infty} \left(\frac{1}{n} \right) \right] \\
 &= \frac{1}{4} (1) \quad \text{RHS}
 \end{aligned}$$

Hence proved.

$$5) \lim_{x \rightarrow 0} \frac{(1+x)^a - 1}{x} = a.$$

from Binomial Expansion, for real number n ,

$$(1+x)^n = \sum_{k=0}^{\infty} \binom{n}{k} x^k \left[\binom{n}{k} = \frac{n(n-1)\dots(n-k+1)}{k!} \right]$$

$$(1+x)^n = 1 + nx + \frac{n(n-1)}{2!}x^2 + \dots$$

Substituting above expansion in our problem with $n=a$;

$$\text{LHS} = \lim_{x \rightarrow 0} \frac{(1+x)^a - 1}{x} = \lim_{x \rightarrow 0} \frac{\left(1 + ax + \frac{a(a-1)}{2!}x^2 + \dots\right) - 1}{x}$$

$$= \lim_{x \rightarrow 0} \frac{1 + \cancel{x} \left(a + \frac{a(a-1)}{2!}x + \dots \right) - 1}{\cancel{x}}$$

wkT,

$$\lim_{x \rightarrow c} f(x) + g(x) = \lim_{x \rightarrow c} f(x) + \lim_{x \rightarrow c} g(x)$$

$$= \lim_{x \rightarrow 0} a + \lim_{x \rightarrow 0} \frac{a(a-1)}{2!}x + \lim_{x \rightarrow 0} \frac{a(a-1)(a-2)}{3!}x^2$$

$$\lim_{x \rightarrow c} \cancel{a} + g(x)f(x) = \lim_{x \rightarrow c} g(x) \cdot \lim_{x \rightarrow c} f(x)$$

$$= a + \frac{a(a-1)}{2} \left(\lim_{x \rightarrow 0} x \right) + \frac{a(a-1)(a-2)}{6} \left(\lim_{x \rightarrow 0} x^2 \right)$$

$$= a + 0 + 0 + 0 \dots = a$$

$$\lim_{x \rightarrow 0} \frac{(1+x)^a - 1}{x} = a = R+1 S.$$

Hence proved

$$\text{8 (a)} \sum_{n=1}^{\infty} u_n, \quad u_n = \left(\frac{a^n}{(n!)^{1/n}} \right)$$

Now again by Cauchy's root test

$\sum u_n$ (i) converges if $\lim_{n \rightarrow \infty} \sqrt[n]{u_n} = l < 1$
 (ii) diverges. Pf $\lim_{n \rightarrow \infty} \sqrt[n]{u_n} = l > 1$

$$\sqrt[n]{n} =$$

$$\frac{a}{(n!)^{1/n^2}}$$

$$\frac{a}{(n \cdot n \cdot n \dots)^{1/n^2}}$$

$$< \frac{a}{(1 \cdot 2 \cdot 3 \cdot 4 \dots n)^{1/n^2}}$$

$$< \frac{a}{(1 \cdot 1 \cdot 1 \cdot 1)^{1/n^2}}$$

So now we have

$$\frac{a}{n^{1/n}} < \frac{a}{\left[1 \cdot 2 \cdot 3 \cdots a\right]^{1/n^2}} < a$$

$$\text{Now } \lim_{n \rightarrow \infty} (n)^{1/n} = 1$$

$$\lim_{n \rightarrow \infty} \left(\frac{a}{n^{1/n}} \right) < \lim_{n \rightarrow \infty} \sqrt[n]{u_n} < \lim_{n \rightarrow \infty} a$$

$$a(1) < \lim_{n \rightarrow \infty} \sqrt[n]{u_n} < a$$

So we have $\lim_{n \rightarrow \infty} \sqrt[n]{u_n} = a$ by

Sandwich theorem

So if $a < 1$ the series will be converging
& if $a > 1$ the series will be diverging

$$8(b) \sum_{n=1}^{\infty} a^n \left(1 + \frac{1}{n}\right)^n$$

in the above series the value of n^{th} term

$$(a_n) = a^n \left(1 + \frac{1}{n}\right)^n$$

applying root test,

$\sum u_n$ (i) converges if $\lim_{n \rightarrow \infty} \sqrt[n]{u_n} = L < 1$
 (ii) diverges if $\lim_{n \rightarrow \infty} \sqrt[n]{u_n} = L > 1$

$$L = \lim_{n \rightarrow \infty} \sqrt[n]{|a_n|} = \lim_{n \rightarrow \infty} \sqrt[n]{a^n \left(1 + \frac{1}{n}\right)^n}$$

$$= \lim_{n \rightarrow \infty} \sqrt[n]{a^n} \cdot \lim_{n \rightarrow \infty} \sqrt[n]{\left(1 + \frac{1}{n}\right)^n}$$

$$= \lim_{n \rightarrow \infty} |a| \cdot \lim_{n \rightarrow \infty} \left(1 + \frac{1}{n}\right)$$

$$L = |a| \cdot 1$$

as we know $a > 0$.

hence, series is convergent if $a < 1$ ($a > 0$)

\therefore convergent if $0 < a < 1$

\Rightarrow series is divergent if $a > 1$

for the case $a = 1$; we cannot conclude nature

of the series for $a = 1$

by applying test for divergence,

$$\lim_{n \rightarrow \infty} a_n = \lim_{n \rightarrow \infty} \left(1 + \frac{1}{n}\right)^n = e$$

$$\sum a_n = \sum 1^n \left(1 + \frac{1}{n}\right)^n = \sum \left(1 + \frac{1}{n}\right)^n$$

wkt,

$$\left(1 + \frac{1}{n}\right)^n > 1$$

$$\forall n \in \mathbb{N}$$

$$\frac{1}{n} > 0$$

$$1 + \frac{1}{n} > 0$$

$$1 + \frac{1}{n} > 1$$

$$\left(1 + \frac{1}{n}\right)^n > (1)^n$$

hence we can say that

$$\sum a_n = \sum \left(1 + \frac{1}{n}\right)^n \text{ is divergent}$$

Since $\lim_{n \rightarrow \infty} a_n \neq 0$

we can conclude series diverges for $a \geq 1$

3. Let us, $\{a_n\}$ not convergent sequence
then according to the definition of convergent
series

$$|a_n - L| \geq \epsilon_0$$

given, $a_n \geq 1$, $a_n + \frac{1}{a_n}$ is convergent

if $a_n \geq 1$ then

$$0 < \frac{1}{a_n} \leq 1$$

$$|a_n + \frac{1}{a_n} - L| > \epsilon_0 - |L - L|$$

according to our assumption:

$$\forall \epsilon_0 > 0 \exists N_0 \in \mathbb{N} \text{ s.t. } \forall n \geq N_0$$

$$|a_n - L| \geq \epsilon_0$$

let us take an $\epsilon_0 > |L - L|$
such that $\epsilon_0 - |L - L| > 0$

$$\text{let, } \epsilon_0 - |L - L| = \epsilon$$

$$\text{then } |a_n + \frac{1}{a_n} - L| > \epsilon$$

But by def convergent series.

$$\forall \epsilon_0 > 0 \exists N_0 \in \mathbb{N} \text{ s.t. } \forall n \geq N_0$$

let $a_n + \frac{1}{a_n}$ converge to L

$$|a_n - L| = |a_n + \frac{1}{a_n} - L + L - L - \frac{1}{a_n}|$$

$$\leq |a_n + \frac{1}{a_n} - L| + |L - L - \frac{1}{a_n}|$$

as

$$0 < \frac{1}{a_n} \leq 1$$

$$< |a_n + \frac{1}{a_n} - L| + |L - L|$$

$$|a_n + \frac{1}{a_n} - L| + |L - L| > \epsilon_0$$

$\forall \epsilon_0 > 0 \exists N_0 \in \mathbb{N}$ s.t. $\forall n \geq N_0$

but $\left| a_n - L \right| < \epsilon_0$

taking $\epsilon_0 < \epsilon$

there will not exist an $N_0 \in \mathbb{N}$

s.t. $\forall n \geq N_0$

the definition does not satisfy

But we know that a_n is
convergent we have reached a
contradiction

$\therefore a_n$ is convergent